refactor

Trie.fst
@@ -6,6 +6,7 @@ module U = FStar.UInt
 
 let alphabet_size : U32.t = U32.uint_to_t 26
 
+// b_nat represents a bounded natural that can fit in 32 bits
 type b_nat = x:nat{x < U32.v alphabet_size /\ U.size x 32}
 
 noeq
@@ -13,9 +14,11 @@ type trie0 (n : U32.t) =
   | L
   | N of raw (trie0 n) n & bool
 
+type trie_array = raw (trie0 alphabet_size) alphabet_size
+
 let empty : trie0 alphabet_size = L
 
-let rec mem (t : trie0 alphabet_size) (l : list b_nat) : Tot bool (decreases l) =
+let rec mem (l : list b_nat) (t : trie0 alphabet_size) : Tot bool (decreases l) =
   match t with
   | L -> false
   | N (a, is_t) ->
@@ -24,21 +27,21 @@ let rec mem (t : trie0 alphabet_size) (l : list b_nat) : Tot bool (decreases l) 
     | x::xs ->
       match index a (U32.uint_to_t x) with
       | L -> false
-      | t' -> mem t' xs
+      | t' -> mem xs t'
 
-let empty_array : raw (trie0 alphabet_size) alphabet_size =
+let empty_array : trie_array =
   init alphabet_size (fun _ -> L)
 
-let rec insert0 (t : trie0 alphabet_size) (l: list b_nat) : Tot (trie0 alphabet_size) (decreases l) =
+let rec insert0 (l: list b_nat) (t : trie0 alphabet_size) : Tot (trie0 alphabet_size) (decreases l) =
   match (t,l) with
   | (L, []) -> N (empty_array, true)
   | (N (a, _), []) -> N (a, true)
-  | (L, x::xs) -> N (init alphabet_size (fun i -> if i = x then insert0 L xs else L), false)
+  | (L, x::xs) -> N (init alphabet_size (fun i -> if i = x then insert0 xs L else L), false)
   | (N (a, b), x::xs) ->
     let t' = index a (U32.uint_to_t x) in
-    N (update a (U32.uint_to_t x) (insert0 t' xs), b)
+    N (update a (U32.uint_to_t x) (insert0 xs t'), b)
 
-let rec is_empty' (a:raw (trie0 alphabet_size) alphabet_size) (i:nat{i < U32.v alphabet_size})
+let rec is_empty' (a:trie_array) (i:b_nat)
   : Tot bool (decreases i)
 = if N? (index a (U32.uint_to_t i))
   then false
@@ -46,10 +49,10 @@ let rec is_empty' (a:raw (trie0 alphabet_size) alphabet_size) (i:nat{i < U32.v a
        then true
        else is_empty' a (i-1)
 
-let is_empty (a:raw (trie0 alphabet_size) alphabet_size) : bool
+let is_empty (a:trie_array) : bool
   = is_empty' a ((U32.v alphabet_size) - 1)
 
-let rec delete0 (t : trie0 alphabet_size) (l: list b_nat) : Tot (trie0 alphabet_size) (decreases l) =
+let rec delete0 (l: list b_nat) (t : trie0 alphabet_size) : Tot (trie0 alphabet_size) (decreases l) =
   match (t,l) with
   | (L, _) -> L
   | (N (a, _), []) -> if is_empty a then L else N (a,false)
@@ -57,7 +60,7 @@ let rec delete0 (t : trie0 alphabet_size) (l: list b_nat) : Tot (trie0 alphabet_
       match index a (U32.uint_to_t x) with
       | L -> N (a, is_t)
       | t' ->
-        match delete0 t' xs with
+        match delete0 xs t' with
         | L -> let N (a',b') = N (update a (U32.uint_to_t x) L , is_t)
                in if is_empty a' && not is_t
                   then L
