TrieInv.fst
@@ -16,90 +16,76 @@ let rec is_trie (t:trie0 alphabet_size) : Tot prop
   match t with
   | L -> true
   | N (a,true) ->
-    (forall (i:nat{i < U32.v alphabet_size}).
+    (forall (i:b_nat).
       is_trie (index a (U32.uint_to_t i)))
   | N (a,false) ->
-    (forall (i:nat{i < U32.v alphabet_size}).
+    (forall (i:b_nat).
       is_trie (index a (U32.uint_to_t i)))
     /\
-    (exists (i:nat{i < U32.v alphabet_size}).
+    (exists (i:b_nat).
         N? (index a (U32.uint_to_t i)))
 
 type trie = t:(trie0 alphabet_size){is_trie t}
 
 // --- Insert Lemmas ---
 
-let insert0_lem (f:(i:nat{i < U32.v alphabet_size}) -> trie0 alphabet_size)
-                (i:nat{i < U32.v alphabet_size})
-  : Lemma (requires (N? (f i)))
-          (ensures N? (index (init alphabet_size f) (U32.uint_to_t i)))
-  = ()
-
 let rec insert0_trie (l:list b_nat) (t:trie0 alphabet_size)
-  : Lemma (requires is_trie t) (ensures is_trie (insert0 t l))
+  : Lemma (requires is_trie t) (ensures is_trie (insert0 l t))
   =
   match (t,l) with
   | (L,[]) -> ()
   | (_,[]) -> ()
-  | (L,x::xs) ->
-    insert0_lem (fun i -> if i = x then insert0 L xs else L) x;
-    insert0_trie xs L
+  | (L,x::xs) -> insert0_trie xs L
   | (N (a, b), x::xs) -> insert0_trie xs (index a (U32.uint_to_t x))
 
 let insert (x:list b_nat) (t:trie) : trie
   =
   insert0_trie x t;
-  insert0 t x
+  insert0 x t
 
 // --- Empty array Lemmas ---
 
 // Forward: exists child node ==> not (is_empty a)
 
-let rec del_lem_back1 (a:raw (trie0 alphabet_size) alphabet_size)
-                      (i':nat{i' < U32.v alphabet_size})
+let rec del_lem_back2 (a:trie_array)
+                      (i':b_nat)
                       (pf:squash (not (is_empty' a i')))
   : Tot (squash (not (is_empty a))) (decreases (U32.v alphabet_size - i'))
   =
   if i' = U32.v alphabet_size - 1
   then pf
   else let pf' : squash (not (is_empty' a (i'+1))) = () in
-       del_lem_back1 a (i'+1) pf'
+       del_lem_back2 a (i'+1) pf'
 
-let del_lem_back (a:raw (trie0 alphabet_size) alphabet_size)
-  : Lemma (requires (exists (i:nat{i < U32.v alphabet_size}).
+let del_lem_back1 (a:trie_array)
+  : Lemma (requires (exists (i:b_nat).
                      N? (index a (U32.uint_to_t i))))
           (ensures not (is_empty a))
   =
-  let pf : squash (exists (i': nat{i' < U32.v alphabet_size}). not (is_empty' a i')) = () in
+  let pf : squash (exists (i': b_nat). not (is_empty' a i')) = () in
   exists_elim
-  #(i':nat{i' < U32.v alphabet_size})
+  #_
   #(fun i' -> not (is_empty' a i'))
   #(not (is_empty a))
   pf
-  (del_lem_back1 a)
+  (del_lem_back2 a)
 
-let del_lem_back' (a:raw (trie0 alphabet_size) alphabet_size)
-  : Lemma ((exists (i:nat{i < U32.v alphabet_size}).
+let del_lem_back (a:trie_array)
+  : Lemma ((exists (i:b_nat).
                     N? (index a (U32.uint_to_t i)))
            ==>
           (not (is_empty a)))
   =
-  implies_intro (exists (i:nat{i < U32.v alphabet_size}).
+  implies_intro (exists (i:b_nat).
                          N? (index a (U32.uint_to_t i)))
                 (fun pfp -> (not (is_empty a)))
-                (fun pfp -> del_lem_back a)
-
-let del_lem_back_neg (a:raw (trie0 alphabet_size) alphabet_size)
-  : Lemma (requires is_empty a)
-          (ensures (forall (i:nat{i < U32.v alphabet_size}).
-                            L? (index a (U32.uint_to_t i))))
-  = del_lem_back' a
+                (fun pfp -> del_lem_back1 a)
 
 // Backward:  exists child node <== not (is_empty a)
 
-let rec del_lem' (a:raw (trie0 alphabet_size) alphabet_size) (i:nat{i < U32.v alphabet_size})
+let rec del_lem' (a:trie_array) (i:b_nat)
   : Lemma (requires not (is_empty' a i))
-          (ensures (exists (i:nat{i < U32.v alphabet_size}).
+          (ensures (exists (i:b_nat).
                             N? (index a (U32.uint_to_t i))))
   =
   if N? (index a (U32.uint_to_t i))
@@ -108,16 +94,16 @@ let rec del_lem' (a:raw (trie0 alphabet_size) alphabet_size) (i:nat{i < U32.v al
       then ()
       else del_lem' a (i-1)
 
-let del_lem (a:raw (trie0 alphabet_size) alphabet_size)
+let del_lem (a:trie_array)
   : Lemma (requires not (is_empty a))
-          (ensures (exists (i:nat{i < U32.v alphabet_size}).
+          (ensures (exists (i:b_nat).
                             N? (index a (U32.uint_to_t i))))
   = del_lem' a (U32.v alphabet_size - 1)
 
 // --- Delete Lemmas ---
 
 let rec delete0_trie (l:list b_nat) (t:trie0 alphabet_size)
-  : Lemma (requires is_trie t) (ensures is_trie (delete0 t l))
+  : Lemma (requires is_trie t) (ensures is_trie (delete0 l t))
   =
   match (t,l) with
   | (L,_) -> ()
@@ -126,7 +112,7 @@ let rec delete0_trie (l:list b_nat) (t:trie0 alphabet_size)
       match index a (U32.uint_to_t x) with
       | L -> ()
       | t' ->
-        match delete0 t' xs with
+        match delete0 xs t' with
         | L -> let N (a',b') = N (update a (U32.uint_to_t x) L , is_t)
                in if is_empty a' && not is_t
                   then ()
@@ -136,4 +122,4 @@ let rec delete0_trie (l:list b_nat) (t:trie0 alphabet_size)
 let delete (x:list b_nat) (t:trie) : trie
   =
   delete0_trie x t;
-  delete0 t x
+  delete0 x t
